checkpoint, incorrect assumption
termination conditions for Lambda need to include affinity
hypotheses. for example, number of beta reductions doesn't
necessarily decrease unless the lambda term is affine.

Affine/Conversion.lean
@@ -16,30 +16,32 @@ def of_lambda {e : Lambda} (h : e.is_affine) : Affine e.free :=
   | .var x => .var x
   | .abs x _ => .abs x (Affine.of_lambda (Lambda.is_affine_of_abs.mp h).1)
   | .app _ _ =>
-    have ⟨he₁, he₂, hinter⟩ := Lambda.is_affine_of_app.mp h
-    .app (Affine.of_lambda he₁) (Affine.of_lambda he₂) hinter
+    .app
+      (Affine.of_lambda (Lambda.is_affine_of_app.mp h).1)
+      (Affine.of_lambda (Lambda.is_affine_of_app.mp h).2.1)
+      (Lambda.is_affine_of_app.mp h).2.2
 
 /-- Conversions preserve free variables. -/
 theorem to_lambda_free_eq (e : Affine vs) : e.free = e.to_lambda.free := by
   match e with
-  | .var x => simp only [free, to_lambda, Lambda.free]
-  | .abs x e => simp only [free, to_lambda, Lambda.free, to_lambda_free_eq e]
+  | .var _ => rfl
+  | .abs _ e => simp only [free, to_lambda, Lambda.free, to_lambda_free_eq e]
   | .app e₁ e₂ h =>
     simp only [free, to_lambda, Lambda.free, to_lambda_free_eq e₁, to_lambda_free_eq e₂]
 
 /-- Conversions preserve counts. -/
 theorem to_lambda_count_eq (e : Affine vs) : e.count x = e.to_lambda.count x := by
   match e with
-  | .var x' => simp only [count, to_lambda, Lambda.count]
-  | .abs x' e => simp only [count, to_lambda, Lambda.count, to_lambda_count_eq e]
+  | .var _ => rfl
+  | .abs _ e => simp only [count, to_lambda, Lambda.count, to_lambda_count_eq e]
   | .app e₁ e₂ h =>
     simp only [count, to_lambda, Lambda.count, to_lambda_count_eq e₁, to_lambda_count_eq e₂]
 
 /-- Conversions preserve affinity. -/
 theorem to_lambda_is_affine (e : Affine vs) : e.to_lambda.is_affine := by
   match e with
-  | .var x => simp only [to_lambda, Lambda.is_affine]
-  | .abs x e =>
+  | .var _ => rfl
+  | .abs _ e =>
     have he := to_lambda_is_affine e
     have hc := Lambda.affine_count_le_one he
     simp only [to_lambda, Lambda.is_affine, he, hc, true_and, decide_True]
@@ -48,17 +50,29 @@ theorem to_lambda_is_affine (e : Affine vs) : e.to_lambda.is_affine := by
       to_lambda_is_affine e₁, to_lambda_is_affine e₂, true_and, decide_eq_true_eq,
       ← to_lambda_free_eq e₁, ← to_lambda_free_eq e₂, h]
 
-theorem to_lambda_count_β_eq (e : Affine vs) : e.to_lambda.count_β = e.count_β := by sorry
-
-theorem of_lambda_count_β_eq {e : Lambda} (h : e.is_affine) :
-    (Affine.of_lambda h).count_β = e.count_β := by sorry
+theorem to_lambda_count_β_eq (e : Affine vs) : e.to_lambda.count_β = e.count_β := by
+  match e with
+  | .var _ => rfl
+  | .abs _ _ => simp only [to_lambda, Lambda.count_β, count_β_of_abs, to_lambda_count_β_eq]
+  | .app (.var _) _ _ =>
+    simp only [to_lambda, Lambda.count_β, count_β_of_app_var, to_lambda_count_β_eq]
+  | .app (.abs _ _) _ _ =>
+    simp only [to_lambda, Lambda.count_β, count_β_of_app_abs, to_lambda_count_β_eq]
+  | .app (.app _ _ _) _ _ =>
+    simp only [to_lambda, Lambda.count_β, count_β_of_app_app, to_lambda_count_β_eq]
 
 end Affine
 
 namespace Lambda
 
-theorem of_lambda_to_lambda {e : Lambda} (h : e.is_affine) :
-    (Affine.of_lambda h).to_lambda = e := by
-  sorry
+theorem of_lambda_to_lambda {e : Lambda} (h : e.is_affine) : (Affine.of_lambda h).to_lambda = e
+    := by
+  match e with
+  | .var _ => rfl
+  | .abs _ e =>
+    simp only [Affine.of_lambda, Affine.to_lambda, abs.injEq, true_and, of_lambda_to_lambda]
+  | .app e₁ e₂ =>
+    simp only [is_affine, decide_eq_true_eq] at h
+    simp only [Affine.of_lambda, Affine.to_lambda, h, of_lambda_to_lambda]
 
 end Lambda
