Affine/Substitution.lean
@@ -1,4 +1,5 @@
 import «Affine».Lemmas
+import «Affine».Misc
 
 namespace Lambda
 
@@ -31,6 +32,8 @@ def substₑ (e₁ : Lambda) (x : ℕ) (e₂ : Lambda) : Lambda :=
       .abs x' (e₁.substₑ x e₂)
 termination_by e₁.depth
 
+theorem substᵥ_count_β {e : Lambda} : (e.substᵥ x y).count_β = e.count_β := by sorry
+
 theorem substₑ_count {e₁ e₂ : Lambda} :
     (e₁.substₑ x' e₂).count x ≤ (if x = x' then 0 else e₁.count x) + e₂.count x := by
   sorry
@@ -58,6 +61,35 @@ theorem is_affine_substₑ {e₁ e₂ : Lambda} (he₁ : e₁.is_affine) (he₂ 
     (e₁.substₑ x e₂).is_affine := by
   sorry
 
-theorem substₑ_count_β {e₁ e₂ : Lambda} : (e₁.substₑ x e₂).count_β < 1 + e₁.count_β + e₂.count_β := by sorry
+theorem substₑ_count_β {e₁ e₂ : Lambda} :
+    (e₁.substₑ x e₂).count_β < 1 + e₁.count_β + e₂.count_β := by
+  match e₁ with
+  | .var x' =>
+    have h₁ : e₂.count_β < 1 + e₂.count_β := lt_one_add _
+    have h₂ : 0 < 1 + e₂.count_β := by simp only [add_pos_iff, zero_lt_one, true_or]
+    simp only [substₑ, count_β, add_zero, apply_ite, ite_lt h₁ h₂]
+
+  | .abs x' e₁ =>
+    simp only [substₑ, count_β, apply_ite count_β]
+    wlog hx₁ : x ∈ e₁.free
+    · simp only [if_pos (Or.inr hx₁), add_assoc, Nat.lt_one_add_iff.mpr, le_add_iff_nonneg_right,
+        zero_le]
+    wlog hxeq : x ≠ x'
+    · simp only [if_pos (Or.inl (not_not.mp hxeq)), add_assoc, Nat.lt_one_add_iff.mpr,
+        le_add_iff_nonneg_right, zero_le]
+    rw [if_neg]
+    by_cases hx' : x' ∈ e₂.free
+    · rw [if_pos hx']
+      have hinc := substₑ_count_β (e₁ := e₁.substᵥ x' e₂.free.fresh) (e₂ := e₂) (x := x)
+      simp [substᵥ_count_β] at hinc
+      exact hinc
+    · simp only [if_neg hx', substₑ_count_β (e₁ := e₁)]
+    simp only [not_or, not_not, hx₁, hxeq, not_false_eq_true, true_and]
+
+  | .app a₁ a₂ =>
+    simp only [substₑ, count_β]
+    have x := count_β_of_app (e₁ := substₑ a₁ x e₂) (e₂ := substₑ a₂ x e₂)
+
+termination_by e₁.depth
 
 end Lambda
